src/op_sem.lean
@@ -1,0 +1,326 @@
+import IMP
+
+open com
+
+inductive big_step : com × pstate → pstate → Prop
+| Skip {s : pstate} : 
+  big_step (SKIP, s) s
+
+| Assign {s : pstate} {x : vname} {a : aexp} : 
+  big_step (x ::= a, s) (s[x ↦ aval a s])
+
+| Seq {c₁ c₂ : com} {s₁ s₂ s₃ : pstate} : 
+  big_step (c₁, s₁) s₂ →
+  big_step (c₂, s₂) s₃ → 
+  big_step (c₁ ;; c₂, s₁) s₃
+
+| IfTrue {b : bexp} {c₁ c₂ : com} {s t : pstate}  : 
+  bval b s →
+  big_step (c₁, s) t → 
+  big_step (IF b THEN c₁ ELSE c₂, s) t
+
+| IfFalse {b : bexp}  {c₁ c₂ : com} {s t : pstate} :
+  ¬ bval b s → 
+  big_step (c₂, s) t →
+  big_step (IF b THEN c₁ ELSE c₂, s) t
+
+| WhileFalse {b : bexp} {c : com} {s : pstate} :
+  ¬ bval b s →
+  big_step (WHILE b DO c, s) s
+
+| WhileTrue {b : bexp} {c : com} {s₁ s₂ s₃ : pstate } :
+  bval b s₁ →
+  big_step (c, s₁) s₂ →
+  big_step (WHILE b DO c, s₂) s₃ →
+  big_step (WHILE b DO c, s₁) s₃
+
+infix ` ⇒ `:70 := big_step
+
+namespace big_step
+
+open big_step
+
+namespace rule_inversion
+
+lemma skip {s t : pstate} (h : (SKIP, s) ⇒ t) : 
+  t = s :=
+begin cases ‹(SKIP, s) ⇒ t›, reflexivity end
+
+lemma assign {x : vname} {a : aexp} {s t : pstate} (h : (x ::= a, s) ⇒ t) : 
+  t = (s[x ↦ aval a s]) :=
+begin cases ‹(x ::= a, s) ⇒ t›, reflexivity end 
+
+lemma seq {c₁ c₂ : com} {s₁ s₃ : pstate} (h : (c₁ ;; c₂, s₁) ⇒ s₃) : 
+  ∃ (s₂ : pstate), (c₁, s₁) ⇒ s₂ ∧ (c₂, s₂) ⇒ s₃ :=
+begin
+  cases ‹(c₁ ;; c₂, s₁) ⇒ s₃›,
+  apply exists.intro,
+  split,
+    exact ‹(c₁, s₁) ⇒ h_s₂›,
+    exact ‹(c₂, h_s₂) ⇒ s₃›
+end
+
+lemma ifte {b : bexp} {c₁ c₂ : com} {s t : pstate} (h : (IF b THEN c₁ ELSE c₂, s) ⇒ t) :
+  (bval b s ∧ (c₁, s) ⇒ t) ∨ (¬bval b s ∧ (c₂, s) ⇒ t) :=
+begin
+  cases ‹(IF b THEN c₁ ELSE c₂, s) ⇒ t›,
+    case IfTrue : { exact or.inl ⟨‹↥(bval b s)›, ‹(c₁, s) ⇒ t›⟩ },
+    case IfFalse : { exact or.inr ⟨‹¬↥(bval b s)›, ‹(c₂, s) ⇒ t›⟩ }
+end
+
+lemma while {b : bexp} {c : com} {s t : pstate} (h : (WHILE b DO c, s) ⇒ t) :
+  (¬bval b s ∧ t = s) ∨ (bval b s ∧ ∃ (s₁ : pstate), (c, s) ⇒ s₁ ∧ (WHILE b DO c, s₁) ⇒ t) :=
+begin
+  cases ‹(WHILE b DO c, s) ⇒ t›,
+    case WhileTrue : { 
+      have : ∃ (s₁ : pstate), (c, s) ⇒ s₁ ∧ (WHILE b DO c, s₁) ⇒ t := 
+        ⟨h_s₂, ⟨‹(c, s) ⇒ h_s₂›, ‹(WHILE b DO c, h_s₂) ⇒ t›⟩⟩,
+      exact or.inr ⟨‹↥(bval b s)›, ‹∃ (s₁ : pstate), (c, s) ⇒ s₁ ∧ (WHILE b DO c, s₁) ⇒ t›⟩ 
+    },
+    case WhileFalse : { exact or.inl ⟨‹¬↥(bval b s)›, rfl⟩ }
+end
+
+end rule_inversion
+
+lemma seq_assoc {c₁ c₂ c₃ : com} {s t : pstate} :
+  (c₁ ;; c₂ ;; c₃, s) ⇒ t ↔ (c₁ ;; (c₂ ;; c₃), s) ⇒ t :=
+begin
+  split,
+    {
+      assume : (c₁ ;; c₂ ;; c₃, s) ⇒ t,
+      have : ∃ s₁, (c₁ ;; c₂, s) ⇒ s₁ ∧ (c₃, s₁) ⇒ t := 
+        rule_inversion.seq ‹(c₁ ;; c₂ ;; c₃, s) ⇒ t›,
+      cases ‹∃ s₁, (c₁ ;; c₂, s) ⇒ s₁ ∧ (c₃, s₁) ⇒ t› with s₁,
+      cases ‹(c₁ ;; c₂, s) ⇒ s₁ ∧ (c₃, s₁) ⇒ t›,
+      have : ∃ s₂, (c₁, s) ⇒ s₂ ∧ (c₂, s₂) ⇒ s₁ := 
+        rule_inversion.seq ‹(c₁ ;; c₂, s) ⇒ s₁›,
+      cases ‹∃ s₂, (c₁, s) ⇒ s₂ ∧ (c₂, s₂) ⇒ s₁› with s₂,
+      cases ‹(c₁, s) ⇒ s₂ ∧ (c₂, s₂) ⇒ s₁›,
+      show (c₁ ;; (c₂ ;; c₃), s) ⇒ t, from
+        Seq ‹(c₁, s) ⇒ s₂› (Seq ‹(c₂, s₂) ⇒ s₁› ‹(c₃, s₁) ⇒ t›)
+    },
+    {
+      assume : (c₁ ;; (c₂ ;; c₃), s) ⇒ t,
+      have : ∃ s₁, (c₁, s) ⇒ s₁ ∧ (c₂ ;; c₃, s₁) ⇒ t :=
+        rule_inversion.seq ‹(c₁ ;; (c₂ ;; c₃), s) ⇒ t›,
+      cases ‹∃ s₁, (c₁, s) ⇒ s₁ ∧ (c₂ ;; c₃, s₁) ⇒ t› with s₁,
+      cases ‹(c₁, s) ⇒ s₁ ∧ (c₂ ;; c₃, s₁) ⇒ t›,
+      have : ∃ s₂, (c₂, s₁) ⇒ s₂ ∧ (c₃, s₂) ⇒ t :=
+        rule_inversion.seq ‹(c₂ ;; c₃, s₁) ⇒ t›,
+      cases ‹∃ s₂, (c₂, s₁) ⇒ s₂ ∧ (c₃, s₂) ⇒ t› with s₂,
+      cases ‹(c₂, s₁) ⇒ s₂ ∧ (c₃, s₂) ⇒ t›,
+      show (c₁ ;; c₂ ;; c₃, s) ⇒ t, from
+        Seq (Seq ‹(c₁, s) ⇒ s₁› ‹(c₂, s₁) ⇒ s₂›) ‹(c₃, s₂) ⇒ t›
+    }
+end
+
+notation c₁ `∼` c₂ := ∀{s t : pstate}, (c₁, s) ⇒ t = (c₂, s) ⇒ t
+
+lemma eq_while_ifwhile {b : bexp} {c : com} : WHILE b DO c ∼ IF b THEN (c ;; WHILE b DO c) ELSE SKIP :=
+begin
+  intros,
+  apply iff.to_eq,
+  split,
+    { 
+      intros,
+      cases ‹(WHILE b DO c, s) ⇒ t›,
+        case WhileFalse : {
+          show  (IF b THEN (c ;; WHILE b DO c) ELSE SKIP, s) ⇒ s, from
+            IfFalse ‹¬↥(bval b s)› Skip
+        },
+        case WhileTrue : {
+          rename ᾰ_s₂ → s',
+          show (IF b THEN (c ;; WHILE b DO c) ELSE SKIP, s) ⇒ t, from
+            IfTrue ‹↥(bval b s)› (Seq ‹(c, s) ⇒ s'› ‹(WHILE b DO c, s') ⇒ t›)
+        }
+    },
+    {
+      intros,
+      cases ‹(IF b THEN (c ;; WHILE b DO c) ELSE SKIP, s) ⇒ t›,
+        case IfTrue : {
+          cases ‹(c ;; WHILE b DO c, s) ⇒ t›,
+          rename ᾰ_ᾰ_1_s₂ → s',
+          show (WHILE b DO c, s) ⇒ t, from
+            WhileTrue ‹↥(bval b s)› ‹(c, s) ⇒ s'› ‹(WHILE b DO c, s') ⇒ t›
+        },
+        case IfFalse : {
+          cases ‹(SKIP, s) ⇒ t›,
+          show (WHILE b DO c, s) ⇒ s, from
+            WhileFalse ‹¬↥(bval b s)›
+        }
+    }
+end
+
+theorem deterministic {c : com} {s : pstate} :
+   ∀{t : pstate}, (c, s) ⇒ t → ∀{r : pstate}, (c, s) ⇒ r → (t = r) :=
+begin
+  assume t : pstate,
+  assume : (c, s) ⇒ t,
+  induction ‹(c, s) ⇒ t›,
+    case Skip : s {
+      assume r : pstate,
+      assume : (SKIP, s) ⇒ r,
+      cases ‹(SKIP, s) ⇒ r›,
+      reflexivity
+    },
+    case Assign : s x a {
+      assume r : pstate,
+      assume : (x ::= a, s) ⇒ r, 
+      cases ‹(x ::= a, s) ⇒ r›,
+      reflexivity
+    },
+    case Seq : c₁ c₂ s s₁ t _ _ ih₁ ih₂ {
+      assume r : pstate,
+      assume : (c₁ ;; c₂, s) ⇒ r,
+      cases ‹(c₁ ;; c₂, s) ⇒ r›, rename this_s₂ → s₂,
+      have : (s₂ = s₁) := (ih₁ ‹(c₁, s) ⇒ s₂›).symm,
+      rw ‹s₂ = s₁› at *,
+      exact ih₂ ‹(c₂, s₁) ⇒ r›
+    },
+    case IfTrue : b c₁ c₂ s _ _ _ ih {
+      assume r : pstate,
+      assume : (IF b THEN c₁ ELSE c₂, s) ⇒ r,
+      cases ‹(IF b THEN c₁ ELSE c₂, s) ⇒ r›,
+        case IfTrue : { exact ih ‹(c₁, s) ⇒ r› },
+        case IfFalse : { contradiction }
+    },
+    case IfFalse : b c₁ c₂ s _ _ _ ih {
+      assume r : pstate,
+      assume : (IF b THEN c₁ ELSE c₂, s) ⇒ r,
+      cases ‹(IF b THEN c₁ ELSE c₂, s) ⇒ r›,
+        case IfTrue : { contradiction },
+        case IfFalse : { exact ih ‹(c₂, s) ⇒ r› }
+    },
+    case WhileTrue : b c s s₁ _ _ _ _ ih₁ ih₂ {
+      assume r : pstate,
+      assume : (WHILE b DO c, s) ⇒ r,
+      cases ‹(WHILE b DO c, s) ⇒ r›,
+        case WhileTrue : { 
+          rename this_s₂ → s₂,
+          have : (s₂ = s₁) := (ih₁ ‹(c, s) ⇒ s₂›).symm,
+          rw ‹s₂ = s₁› at *,
+          exact ih₂ ‹(WHILE b DO c, s₁) ⇒ r›
+        },
+        case WhileFalse : { contradiction }
+    },
+    case WhileFalse : b c s {
+      assume r : pstate,
+      assume : (WHILE b DO c, s) ⇒ r,
+      cases ‹(WHILE b DO c, s) ⇒ r›,
+        case WhileTrue : { contradiction },
+        case WhileFalse : { reflexivity }
+    }
+end
+
+end big_step
+
+inductive small_step : com × pstate → com × pstate → Prop
+| Assign  {s : pstate} {x : vname} {a : aexp} :
+  small_step (x ::= a, s) (SKIP, s[x ↦ aval a s])
+
+| Seq1 {c₂ : com} {s : pstate} :
+  small_step (SKIP;;c₂, s) (c₂, s)
+
+| Seq2 {c₁ c₁' c₂ : com} {s s' : pstate} :
+  small_step (c₁, s) (c₁', s') →
+  small_step (c₁ ;; c₂, s) (c₁';;c₂, s)
+
+| IfTrue {b : bexp} {s : pstate} {c₁ c₂ : com}:
+  bval b s →
+  small_step (IF b THEN c₁ ELSE c₂, s) (c₁, s)
+
+| IfFalse {b : bexp} {s : pstate} {c₁ c₂ : com}:
+  ¬bval b s →
+  small_step (IF b THEN c₁ ELSE c₂, s) (c₂, s)
+
+| While {b : bexp} {c : com} {s : pstate} :
+  small_step (WHILE b DO c, s) (IF b THEN (c ;; WHILE b DO c) ELSE SKIP, s)
+
+infix `↝`:70 := small_step
+
+namespace small_step
+
+open small_step
+
+inductive small_step_star : com × pstate → com × pstate → Prop
+| refl {c : com} {s : pstate} : small_step_star (c, s) (c, s)
+
+| step {c c₁ c₂ : com} {s s₁ s₂ : pstate}:
+  small_step (c, s) (c₁, s₁) →
+  small_step_star (c₁, s₁) (c₂, s₂) →
+  small_step_star (c, s) (c₂, s₂)
+
+infix `↝*`:70 := small_step_star
+
+namespace trans
+
+open small_step_star
+
+@[trans] lemma small_step_star_small_step_star_trans {st st₁ st₂: com × pstate} :
+  st ↝* st₁ → st₁ ↝* st₂ → st ↝* st₂ :=
+begin
+  cases st with c s,
+  cases st₁ with c₁ s₁,
+  cases st₂ with c₂ s₂,
+  intros,
+  induction ‹(c, s)↝*(c₁, s₁)›,
+    case refl : c s { exact ‹(c, s)↝*(c₂, s₂)› },
+    case step : c c₃ c₁ s s₃ s₁  _ _ ih {
+      have : (c₃, s₃)↝*(c₂, s₂) := ih ‹(c₁, s₁)↝*(c₂, s₂)›,
+      exact step ‹(c, s)↝(c₃, s₃)› ‹(c₃, s₃)↝*(c₂, s₂)›
+    }
+end
+
+@[trans] lemma small_step_star_small_step_trans {st st₁ st₂: com × pstate} :
+  st ↝* st₁ → st₁ ↝ st₂ → st ↝* st₂ :=
+begin
+  cases st with c s,
+  cases st₁ with c₁ s₁,
+  cases st₂ with c₂ s₂,
+  intros,
+  induction ‹(c, s)↝*(c₁, s₁)›,
+    case refl : c s { exact step ‹(c, s)↝(c₂, s₂)› refl },
+    case step : c c₃ c₁ s s₃ s₁ _ _ ih {
+      have : (c₃, s₃)↝*(c₂, s₂) := ih ‹(c₁, s₁)↝(c₂, s₂)›,
+      exact step ‹(c, s)↝(c₃, s₃)› ‹(c₃, s₃)↝*(c₂, s₂)›
+    }
+end 
+
+@[trans] lemma small_step_small_step_star_trans {st st₁ st₂: com × pstate} :
+  st ↝ st₁ → st₁ ↝* st₂ → st ↝* st₂ :=
+begin
+  cases st with c s,
+  cases st₁ with c₁ s₁,
+  cases st₂ with c₂ s₂,
+  intros,
+  exact step ‹(c, s)↝(c₁, s₁)› ‹(c₁, s₁)↝*(c₂, s₂)›
+end
+
+@[trans] lemma small_step_small_step_trans {st st₁ st₂: com × pstate} :
+  st ↝ st₁ → st₁ ↝ st₂ → st ↝* st₂ :=
+begin
+  cases st with c s, 
+  cases st₁ with c₁ s₁,
+  cases st₂ with c₂ s₂,
+  intros,
+  have : (c₁, s₁)↝*(c₁, s₁) := refl,
+  have : (c, s)↝*(c₁, s₁) := step ‹(c, s)↝(c₁, s₁)› ‹(c₁, s₁)↝*(c₁, s₁)›,
+  exact small_step_star_small_step_trans ‹(c, s)↝*(c₁, s₁)› ‹(c₁, s₁)↝(c₂, s₂)›
+end
+
+end trans
+
+/-
+constant s : state
+constant p : ↥(bval (Bc tt) s) 
+example : (IF (Bc tt) THEN SKIP ;; SKIP ELSE SKIP, s)↝*(SKIP, s) :=
+  calc
+    (IF (Bc tt) THEN SKIP ;; SKIP ELSE SKIP, s)↝(SKIP ;; SKIP, s) : 
+      small_step.IfTrue p
+    ...                                        ↝(SKIP, s)         : 
+      small_step.Seq1
+    ...                                        ↝*(SKIP, s)        :
+      small_step_star.refl 
+-/
+
+end small_step
